Earley/Proofs/Finiteness.lean
@@ -51,13 +51,13 @@ Due the WellFormed-constraints, this results in a Product Set `Top` of
 The members of the Product are all individually finite, therefore the Product is also finite.
 Since the well-formed EarleyItems are simply a subset of this `Top`, that set also has to be finite.
 -/
-public theorem finiteEarleyNonEmpty (G : ContextFreeGrammarList T N) (w : List (Symbol T N))
-    (hempty : G.rules ≠ []) : Finite { x | isWellFormed G.rules w x } := by
+public theorem finiteEarleyNonEmpty (G : ContextFreeGrammarList T N) (wlen : Nat)
+    (hempty : G.rules ≠ []) : Finite { x | isWellFormed G.rules wlen x } := by
   -- The maximum length of any rule
   let M := G.rules.map (fun r => r.output.length) |>.max (by simp [hempty])
   let ruleSet := {x | x ∈ G.rules}
   -- The Set of all possible assignments of an EarleyItem with bounded rule length
-  let Top := ruleSet ×ˢ ({i | i ≤ M} ×ˢ  ({i | i ≤ w.length} ×ˢ {i | i ≤ w.length}))
+  let Top := ruleSet ×ˢ ({i | i ≤ M} ×ˢ  ({i | i ≤ wlen} ×ˢ {i | i ≤ wlen}))
   -- The product of four Finite Sets has to be finite as well.
   have finTop : Finite Top := by
     have hFinMem: Finite ruleSet := by
@@ -66,10 +66,10 @@ public theorem finiteEarleyNonEmpty (G : ContextFreeGrammarList T N) (w : List (
       infer_instance
     infer_instance
   have finImageTop: Finite (Top.image itemIntro) := Finite.Set.finite_image Top itemIntro
-  have : { x | isWellFormed G.rules w x } ⊆ Top.image itemIntro := by
+  have : { x | isWellFormed G.rules wlen x } ⊆ Top.image itemIntro := by
     intro x hmemx
     have : x.position ≤ M := by
-      have wf : isWellFormed G.rules w x := by grind
+      have wf : isWellFormed G.rules wlen x := by grind
       simp only [isWellFormed] at wf
       have ⟨hmem,hpos,hs,he⟩ := wf
       have : x.rule.output.length ≤ M := by
@@ -83,8 +83,8 @@ public theorem finiteEarleyNonEmpty (G : ContextFreeGrammarList T N) (w : List (
 /--
 There is only a finite number of well-formed EarleyItems for a specific grammar and word.
 -/
-public theorem finiteEarleyWF (G : ContextFreeGrammarList T N) (w : List (Symbol T N)) :
-    Finite { x | isWellFormed G.rules w x} := by
+public theorem finiteEarleyWF (G : ContextFreeGrammarList T N) (wlen : Nat) :
+    Finite { x | isWellFormed G.rules wlen x} := by
   cases h : G.rules
   · simp [isWellFormed]
     grind [Finite.exists_equiv_fin, Finite.of_fintype]
@@ -99,12 +99,12 @@ but this also showcases some annoyance with CFG vs CFGList that I need to work a
 public theorem finiteEarley (G : ContextFreeGrammar T) [BEq G.NT] (w : List (Symbol T G.NT)) :
     Finite (EarleySet G w) := by
   have hwf := wfEarley G w
-  have hsub : EarleySet G w ⊆ { x | isWellFormed G.rules w x } := by grind
+  have hsub : EarleySet G w ⊆ { x | isWellFormed G.rules w.length x } := by grind
   have : G.rules.toList.Nodup := Finset.nodup_toList G.rules
   let G' : ContextFreeGrammarList T G.NT := ⟨G.initial, G.rules.toList, this⟩
-  have hsub' : EarleySet G w ⊆ { x | isWellFormed G'.rules w x } := by
+  have hsub' : EarleySet G w ⊆ { x | isWellFormed G'.rules w.length x } := by
     grind [Finset.mem_toList]
-  have hf := finiteEarleyWF G' w
+  have hf := finiteEarleyWF G' w.length
   exact Set.Finite.subset hf hsub'
 
 end Finiteness
