Earley/Proofs/Recognizer.lean
@@ -354,7 +354,7 @@ theorem eqItems_of_earleyBinList_of_eqItems {G : ContextFreeGrammarList T N} {w 
         apply eqItems_of_completeList_of_eqItems
         exact heq
       apply eqItems_of_updateBins_of_eqItems heq this
-termination_by { x | isWellFormed G.rules (mapT w) x }.ncard + 1 - j
+termination_by { x | isWellFormed G.rules w.length x }.ncard + 1 - j
 decreasing_by
   all_goals
   exact decreasingAux hbins1 j k hk (by lia)
