EarleyTest/Basic.lean
@@ -126,25 +126,25 @@ theorem finished3 : isFinished G.initial exW1 exItem3 = false := rfl
 theorem finished4 : isFinished G.initial exW1 exItem4 = false := rfl
 theorem finished5 : isFinished G.initial exW1 exItem5 = true := rfl
 
-theorem wf1 : isWellFormed G.rules exW1 exItem1 := by
+theorem wf1 : isWellFormed G.rules exW1.length exItem1 := by
   rw [isWellFormed, exItem1]
   unfold G
   unfold exRules
   simp
 
-theorem wf2 : ¬isWellFormed G.rules exW1 exItem2 := by
+theorem wf2 : ¬isWellFormed G.rules exW1.length exItem2 := by
   rw [isWellFormed, exItem2, exW1]
   simp [List.length]
 
-theorem wf3 : ¬isWellFormed G.rules exW2 exItem3 := by
+theorem wf3 : ¬isWellFormed G.rules exW2.length exItem3 := by
   rw [isWellFormed, exItem3]
   simp
 
-theorem wf4 : ¬isWellFormed G.rules exW2 exItem4 := by
+theorem wf4 : ¬isWellFormed G.rules exW2.length exItem4 := by
   rw [isWellFormed, exItem4, exItem1, exW2, exRule2]
   simp [List.length]
 
-theorem wf5 : isWellFormed G.rules exW2 exItem5 := by
+theorem wf5 : isWellFormed G.rules exW2.length exItem5 := by
   rw [isWellFormed, exItem5, exW2]
   unfold G
   unfold exRules
